Compiles again aftes restructoring

SAMLProtocol.fst
@@ -1,5 +1,9 @@
-module PROTOCOL
+module Protocol
 
+(*TODO: 
+- Gør beskrder endnu mere generelle
+- Så de afspejler http og model bedre 
+*)
 type prin
 type dsig
 type resource
@@ -10,37 +14,19 @@ type samlmessage =
   | AuthnRequest: samlmessage
   | Response: samlmessage
 
-type request =
-  | HttpGet: uri -> request
-  | SamlAuthnRequest: uri -> prin -> samlmessage -> dsig -> string -> request
-  | AuthenticateUser: prin -> string -> string -> nonce -> request
+type message =
+  | HttpGet: uri -> message
+  | SamlProtocolMessage: prin -> samlmessage -> dsig -> string -> message
+  | Credentials: string -> string -> nonce -> message
+  | Challenge: nonce -> message
+  | Resource: uri -> message
+  | Failed: message
 
-type response =
-  | SamlAuthnRequestRedirect: uri -> prin -> samlmessage -> dsig -> string -> response
-  | Challenge: nonce -> response
-  | Failed: response
-
-val send: prin -> request -> unit
-val recieve: prin -> response 
-
+val send: prin -> message -> unit
+val recieve: prin -> message 
 
 val createAuthnRequest: prin -> prin -> (samlmessage * dsig)
-val createChallenge: prin -> string
+val createChallenge: prin -> nonce
 val createSamlResponse: prin -> prin -> (samlmessage * dsig)
 
-val recieveHttpRequest: prin -> uri
-val recieveHttpResponse: prin -> resource
-val recieveAutenticationRequestChallenge: prin -> string
-val recieveAutenticationRequest: prin -> (string * string * string)
-val recieveAutenticationCredentials: prin -> (samlmessage * dsig * string)
-val recievehttpRedirect: prin -> (prin * samlmessage * dsig * string)
-
-val sendRequestResource: prin -> request -> unit
-val sendhttpRedirect: prin -> prin -> samlmessage -> dsig -> string -> unit
-val sendAuthnRequest: prin -> samlmessage -> dsig -> string -> unit
-val sendAutenticationRequest: prin -> string -> string -> string -> unit
-val sendAutenticationChallenge: prin -> string -> unit
-val sendAuthentication: prin -> samlmessage -> string -> unit
-val sendResource: prin -> resource
-
-end (*PROTOCOL*)
+end (*Protocol*)
