identityprovider.fst
@@ -1,5 +1,5 @@
-module IDENTITYPROVIDER
-open PROTOCOL
+module Identityprovider
+open Protocol
 
 (*
 - Protocol events
@@ -9,12 +9,20 @@ open PROTOCOL
 
 val identityprovider: me:prin -> client:prin -> sp:prin -> unit
 let identityprovider me client serviceprovider =
-  let (authnReq, sigSP, relay) = recieveAutenticationRequest client in (*3*)
+	let authRequest = recieve client in (*3*)
+	match authRequest with
+	| SamlProtocolMessage (idp, message, sigSP, relay)-> 
     let challenge = createChallenge client in
-      sendAutenticationChallenge client challenge; (*4*)
-      let (user,password, challenge') = recieveAutenticationCredentials client in (*5*)
-        let (samlResponse, sigIDP) = createSamlResponse me serviceprovider in 
-          sendhttpRedirect client serviceprovider samlResponse sigIDP; (*6*)
-          ()
+    let challengeMessage = Challenge challenge in
+    send client challengeMessage; (*4*)
+    let credentials = recieve client in (*5*)
+      match credentials with
+      | Credentials(user, password, challenge') -> 
+        let (samlresponse, sigIDP) = createSamlResponse me serviceprovider in
+        let response = SamlProtocolMessage serviceprovider samlresponse sigIDP relay in
+        send client response(*6*)
+      | _ -> ()
+	| _ -> ()
+()
 
-end (*IDENTITYPROVIDER*)
+end (*Identityprovider*)
