client.fst
@@ -1,5 +1,5 @@
-module CLIENT
-open PROTOCOL
+module Client
+open Protocol
 
 (*
 - Protocol events
@@ -7,30 +7,28 @@ open PROTOCOL
 - Add asserts
   *)
 
-val client: sp:prin -> req:request -> user:string -> password:string -> unit
+val client: sp:prin -> req:message -> user:string -> password:string -> unit
 let client sp req user password = 
     let _ = send sp req in(*1*)
       let res = recieve sp in(*2*)
         match res with
-        | SamlAuthnRequestRedirect (uri, idp, authnRequest, sigSP, relayState) -> 
-          let samlAuthnReq = SamlAuthnRequest uri idp authnRequest sigSP relayState in
-            send idp samlAuthnReq (*3*)
-            let chal = recieve idp in (*4*)
-              let authUserReq = AutnenticateUser idp user password chal (*6*)
-
-
+        | SamlProtocolMessage (idp, authnRequest, sigSP, relayState) -> 
+          let samlAuthnReq = SamlProtocolMessage idp authnRequest sigSP relayState in
+              send idp samlAuthnReq;
+              let chal = recieve idp in (*4*)
+              match chal with
+              | Challenge (challenge) -> 
+                  let authUserReq = Credentials user password challenge in (*5*)
+                  send idp authUserReq; (*5*)
+                  let idpResp = recieve idp in
+                  match idpResp with
+                  | SamlProtocolMessage (sp', samlResponse, sigIDP, relayState') -> 
+                    let samlResponseRequest =  SamlProtocolMessage sp' samlResponse sigIDP relayState' in (*7*)
+                    send sp' samlResponseRequest;
+                    let resource = recieve sp' in(*8*)
+                    ()
+                  | _ -> ()
+              | _ -> ()
         | _ -> ()
-        
 
-
-(*let client sp req user password = 
-    let _ = send sp req in(*1*)
-      let (idp, authnRequest, sigSP, relayState) = recievehttpRedirect sp in(*2*)
-        sendAuthnRequest idp authnRequest sigSP relayState;(*3*)
-        let challenge = recieveAutenticationRequestChallenge idp in(*4*)
-          sendAutenticationRequest idp user password challenge; (*5*)
-          let (sp', samlResponse, sigIDP, relayState') = recievehttpRedirect idp in(*6*)
-            sendAuthentication sp' samlResponse relayState'; (*7*)
-            let res = recieveHttpResponse sp' in (*8*)
-            ()
-end CLIENT*)
+end (*Client*)
